thy/Routing/IpRoute_Parser.thy
@@ -3,10 +3,11 @@ imports Main "../Primitive_Matchers/IpAddresses" "../Routing/Routing"
 keywords "parse_ip_route" :: thy_decl
 begin
 
-definition "empty_rr_hlp pm = routing_rule.make pm (Port '''') None default_metric"
-lemma empty_rr_hlp_alt: "empty_rr_hlp pm = \<lparr> routing_match = pm, output_iface = Port '''', next_hop = None, metric = 0 \<rparr>"
-unfolding empty_rr_hlp_def routing_rule.defs default_metric_def ..
-definition "update_nh h pk = next_hop_update (const $ Some h) (pk::routing_rule)" 
+definition "empty_rr_hlp pm = routing_rule.make pm default_metric (routing_action.make '''' None)"
+lemma empty_rr_hlp_alt: "empty_rr_hlp pm = \<lparr> routing_match = pm, metric = 0, routing_action = \<lparr>output_iface = [], next_hop = None\<rparr>\<rparr>"
+unfolding empty_rr_hlp_def routing_rule.defs default_metric_def routing_action.defs ..
+definition "routing_action_next_hop_update h pk = routing_action_update (next_hop_update (const $ Some h)) (pk::routing_rule)"
+definition "routing_action_oiface_update h pk = routing_action_update (output_iface_update (const h)) (pk::routing_rule)"
 
 (* Hide all the ugly ml in a file with the right extension *)
 ML_file "IpRoute_Parser.ml"
